Test/civl/large-samples/stack-lemmas.bpl
@@ -1,0 +1,33 @@
+// RUN: %parallel-boogie -lib:base -lib:node "%s" > "%t"
+// RUN: %diff "%s.expect" "%t"
+
+implementation StackAbsCompute<V>(start: Option Loc, nodes: Map (One Loc) (Node V), nodes': Map (One Loc) (Node V)) returns (absStack: Vec V)
+{
+  var loc_n: Option Loc;
+  var n: Node V;
+
+  if (start == None()) {
+      absStack := Vec_Empty();
+  } else {
+      loc_n := start;
+      assert Map_Contains(nodes, One(loc_n->t));
+      n := Map_At(nodes, One(loc_n->t));
+      // Use well-founded list reachability to prove that recursion will terminate:
+      // start@caller --> start@callee --> None()
+      assert Between(nodes->val, loc_n, n->next, None());
+      call absStack := StackAbsCompute(n->next, nodes, nodes');
+      absStack := Vec_Append(absStack, n->val);
+  }
+}
+
+implementation StackAbsLemma<V>(start: Option Loc, nodes: Map (One Loc) (Node V))
+{
+  var absStack: Vec V;
+  call absStack := StackAbsCompute(start, nodes, nodes);
+}
+
+implementation StackFrameLemma<V>(start: Option Loc, nodes: Map (One Loc) (Node V), nodes': Map (One Loc) (Node V))
+{
+  var absStack: Vec V;
+  call absStack := StackAbsCompute(start, nodes, nodes');
+}
